

$$
\lim_{ x \to 0 } \frac{\sqrt{ x } + \sqrt[4]{ x } + x}{\sqrt{ x + 1} - 1}  
$$

$$
\begin{gathered}
\lim_{ x \to 1 } \left( \frac{1}{x^2-x} - \frac{3}{x^3 - 1} \right)  = \lim_{ x \to 1 } \left( \frac{1}{x(x-1)} - \frac{1}{(x-1)(x^2+x+1)} \right) =  \\
=\lim_{ x \to 1 } \left( \frac{x^2+x+1}{x(x-1)(x^2+x+1)} - \frac{3x}{x(x-1)(x^2+x+1)} \right) = \\
= \lim_{ x \to 1 } \left( \frac{(x-1)^2}{x(x-1)(x^2+x+1)} \right) = \lim_{ x \to 1 } = \left(\frac{x-1}{x(x^2+x+1)} \right)  = \\
= \frac{1 - 1}{1(1 + 1 + 1)} = \frac{0}{3} = 0
\end{gathered}
$$
$$
\lim_{ x \to 1 } \frac{(x-1)^8}{x^8-1}
$$
$$
\begin{gathered}
\lim_{ x \to 1 } \frac{(x-1)^8}{x^8-1} = \lim_{ x \to 1 } \frac{(x-1)^8}{(x-1)(x^7+x^6+x^5+x^4+x^3+x^2+x+1)} = \\
\lim_{ x \to 1 } \frac{(x-1)^7}{x^7+x^6+x^5+x^4+x^3+x^2+x+1}  = \frac{0}{8}
\end{gathered}
$$

$$
\lim_{ x \to 0 } \frac{\sin 4x}{\sqrt{ x+1 } - 1} 
$$
$$
\begin{gathered}
\lim_{ x \to 0 } \frac{\sin 4x}{\sqrt{ x+1 } - 1}  = \lim_{ x \to 0 } \frac{\sin 4x}{\sqrt{ x+1 } - 1} \cdot \frac{\sqrt{ x+1 }+1}{\sqrt{ x+1 }+1} = \\
= \lim_{ x \to 0 } \frac{\sin 4x(\sqrt{ x+1 }+1)}{(\sqrt{ x+1 } + 1)(\sqrt{ x+1 } + 1)} = \lim_{ x \to 0 } \frac{\sin 4x \cdot (\sqrt{ x+1 }+1)}{x} = \\
= \lim_{ x \to 0 } \frac{\sin 4x}{x} \cdot \lim_{ x \to 0 } {(\sqrt{ x+1 } + 1)} = 4 \cdot 2 = 8
\end{gathered}
$$

$$
e^x \cdot \sqrt{ 1-e^{2x} } + \arcsin e^x
$$
$$
f'(x) = \frac{2e^x(1-e^{2x})}{\sqrt{ 1-e^{2x} }}
$$

$$
\tan^2 \left( \frac{x+1}{\sqrt{ x }} \right)
$$
$$
  

f{\prime}(x) = \tan\left( \frac{x+1}{\sqrt{x}} \right) \cdot \sec^2\left( \frac{x+1}{\sqrt{x}} \right) \cdot \frac{x - 1}{x\sqrt{x}}.
$$
$$
x^{2\sqrt{ \ln x }}
$$

$$
f{\prime}(x) = x^{2\sqrt{\ln x} - 1} \cdot \frac{\ln x + 2\sqrt{\ln x}}{\sqrt{\ln x}}.
$$
